src/cursor.v
@@ -1,0 +1,136 @@
+(*===========================================================================
+    In order to formalize memory ranges, and reading the very last byte in
+    memory, we introduce a type of Cursor, which is either an actual
+    address or the address beyond the top of memory. In other words, this is
+    just [0..2^n] where n is the number of bits in an address.
+  ===========================================================================*)
+Require Import Ssreflect.ssreflect Ssreflect.ssrfun Ssreflect.ssrnat Ssreflect.ssrbool Ssreflect.finfun Ssreflect.eqtype Ssreflect.fintype Ssreflect.tuple Ssreflect.seq.
+Require Import Ssreflect.choice Ssreflect.tuple Ssreflect.div.
+Require Import bitsrep bitsops.
+
+Set Implicit Arguments.
+Unset Strict Implicit.
+Import Prenex Implicits.
+
+Section Cursors.
+
+(*=Cursor *)
+Variable n:nat.
+Inductive Cursor := mkCursor (p: BITS n) | top.
+(*=End *)
+
+(* Embedding into nat -- for proofs only! *)
+Definition cursorToNat pos := if pos is mkCursor p then toNat p else 2^n.
+
+(*---------------------------------------------------------------------------
+    next: BITS n -> Cursor n
+    and its properties
+  ---------------------------------------------------------------------------*)
+Definition next (p:BITS n) := if p == ones _ then top else mkCursor (incB p).
+
+Definition nextCursor (p:Cursor) :=
+  if p is mkCursor pos then next pos else top.
+
+(*---------------------------------------------------------------------------
+    Order relations on Cursor
+  ---------------------------------------------------------------------------*)
+Definition ltCursor (pos1 pos2: Cursor) :=
+  match pos1, pos2 with
+  | top, _ => false
+  | mkCursor p1, mkCursor p2 => ltB p1 p2
+  | mkCursor _, top => true
+  end.
+Definition leCursor (pos1 pos2: Cursor) :=
+  match pos1, pos2 with
+  | _, top => true
+  | top, mkCursor _ => false
+  | mkCursor p1, mkCursor p2 => leB p1 p2
+  end.
+
+Fixpoint nexts k (c: Cursor) : option (Cursor) :=
+  match k , c with
+  | 0 , _ => Some c
+  | k'.+1 , mkCursor p => nexts k' (next p)
+  | k'.+1 , top => None
+  end.
+
+(*---------------------------------------------------------------------------
+    Apart by n
+  ---------------------------------------------------------------------------*)
+Fixpoint apart n (p q: Cursor) :=
+  match n, p with
+  | n'.+1, mkCursor p' => apart n' (next p') q (* q = next (p' +# n)  *)
+  | 0, _ => q = p
+  | _, _ => False
+  end.
+
+(*---------------------------------------------------------------------------
+    Subtraction
+  ---------------------------------------------------------------------------*)
+Definition subCursor (p q: Cursor) : Cursor :=
+  match p, q with
+  | _, top => mkCursor (zero _)
+  | mkCursor p', mkCursor q' =>
+    if leB p' q' then mkCursor (zero _) else mkCursor (subB p' q')
+  | top, mkCursor p' =>
+    if p' == zero _ then top else mkCursor (negB p')
+  end.
+
+(*---------------------------------------------------------------------------
+    Range testing
+  ---------------------------------------------------------------------------*)
+Definition inRange p q := fun p' => leCursor p p' && ltCursor p' q.
+Definition outRange p q := fun p' => ltCursor p' p && leCursor q p'.
+
+End Cursors.
+
+Coercion mkCursor : BITS >-> Cursor.
+
+(** Convenience definitions for various sizes of cursor *)
+(*Definition NIBBLECursor := Cursor n4.
+Definition BYTECursor   := Cursor n8.
+Definition WORDCursor   := Cursor n16.*)
+Definition DWORDCursor  := Cursor n32.
+(*Definition QWORDCursor  := Cursor n64.
+Definition DWORDorBYTECursor (d: bool) := Cursor (if d then n32 else n8).*)
+
+(*Coercion mkNIBBLECursor (x: NIBBLE) : NIBBLECursor := mkCursor x.
+Coercion mkBYTECursor   (x: BYTE)   : BYTECursor   := mkCursor x.
+Coercion mkWORDCursor   (x: WORD)   : WORDCursor   := mkCursor x.
+Coercion mkDWORDCursor  (x: DWORD)  : DWORDCursor  := mkCursor x.
+Coercion mkQWORDCursor  (x: QWORD)  : QWORDCursor  := mkCursor x.
+Coercion mkDWORDorBYTECursor d (x: DWORDorBYTE d) : DWORDorBYTECursor d := mkCursor x.*)
+
+Identity Coercion DWORDCursortoCursor32 : DWORDCursor >-> Cursor.
+
+Definition widenCursor n1 n2 (c: Cursor n1) : Cursor (n2+n1) :=
+  if c is mkCursor p then mkCursor (p ## zero n2) else top _.
+
+(* Because Cursor is essentially isomorphic to option, we can inherit
+   many canonical structures. *)
+Section CursorCanonicals.
+  Variable n: nat.
+
+  Definition cursor_option (p: Cursor n) : option (BITS n) :=
+    if p is mkCursor p' then Some p' else None.
+
+  Definition option_cursor (o: option (BITS n)) : Cursor n :=
+    if o is Some p' then mkCursor p' else top n.
+
+  Lemma cursor_optionC: cancel cursor_option option_cursor.
+  Proof. by move=> [p|] /=. Qed.
+
+  Definition Cursor_eqMixin := CanEqMixin cursor_optionC.
+  Canonical Structure Cursor_eqType :=
+    Eval hnf in EqType (Cursor n) Cursor_eqMixin.
+
+  Definition Cursor_countMixin := CanCountMixin cursor_optionC.
+  Definition Cursor_choiceMixin := CountChoiceMixin Cursor_countMixin.
+  Canonical Structure Cursor_choiceType :=
+    Eval hnf in ChoiceType _ Cursor_choiceMixin.
+  Canonical Structure Cursor_countType :=
+    Eval hnf in CountType _ Cursor_countMixin.
+
+  Definition Cursor_finMixin := Eval hnf in CanFinMixin cursor_optionC.
+  Canonical Structure Cursor_finType := Eval hnf in FinType _ Cursor_finMixin.
+End CursorCanonicals.
