src/reader.v
@@ -1,0 +1,205 @@
+(*===========================================================================
+    Reader monad, with instances for BYTE, WORD and DWORD
+  ===========================================================================*)
+Require Import Ssreflect.ssreflect Ssreflect.ssrfun Ssreflect.ssrbool Ssreflect.finfun Ssreflect.fintype Ssreflect.ssrnat Ssreflect.eqtype Ssreflect.seq Ssreflect.tuple.
+Require Import bitsrep bitsops monad cursor.
+Require Import Coq.Logic.FunctionalExtensionality Coq.Strings.String. (* x86proved.cstring. *)
+
+Set Implicit Arguments.
+Unset Strict Implicit.
+Import Prenex Implicits.
+
+(* Term representation for a T-reader *)
+(*=Reader *)
+Inductive ReaderTm T :=
+| readerRetn (x: T)
+| readerNext (rd: BYTE -> ReaderTm T)
+| readerSkip (rd: ReaderTm T)
+| readerCursor (rd: DWORDCursor -> ReaderTm T).
+
+Class Reader T := getReaderTm : ReaderTm T.
+(*=End *)
+Instance readCursor : Reader (DWORDCursor) := readerCursor (fun p => readerRetn p).
+Definition readNext {T} {R: Reader T}: Reader T := R.
+
+Fixpoint readerBind X Y (r: Reader X) (f: X -> Reader Y) : Reader Y :=
+  match r with
+  | readerRetn r => f r
+  | readerNext rd => readerNext (fun b => readerBind (rd b) f)
+  | readerSkip rd => readerSkip (readerBind rd f)
+  | readerCursor rd => readerCursor (fun p => readerBind (rd p) f)
+  end.
+
+Fixpoint readerTmSkipFree X (r: ReaderTm X) :=
+match r with
+| readerRetn _ => True
+| readerSkip _ => False
+| readerNext r => forall b, readerTmSkipFree (r b)
+| readerCursor r => forall f, readerTmSkipFree (r f)
+end.
+
+
+Instance readerMonadOps : MonadOps Reader :=
+{ retn := readerRetn
+; bind := readerBind }.
+
+Instance readerMonad : Monad Reader.
+Proof. apply Build_Monad.
+(* id_l *)
+  move => X Y x f. done.
+(* id_r *)
+  move => X. elim => //.
+  - move => rd IH/=.
+    apply f_equal. apply functional_extensionality => b. apply IH.
+  - move => rd IH/=. by apply f_equal.
+  - move => rd IH/=.
+    apply f_equal. apply functional_extensionality => b. apply IH.
+(* assoc *)
+  move => X Y Z. elim => //.
+  - move => rd IH f g/=.
+    apply f_equal. apply functional_extensionality => b. apply IH.
+  - move => rd IH f g/=. by apply f_equal.
+  - move => rd IH f g/=.
+    apply f_equal. apply functional_extensionality => b. apply IH.
+Qed.
+
+(* Functional interpretation of reader on sequences.
+   Returns the final position, the tail of the given sequence and the value
+   read. *)
+Fixpoint runReader T (r:Reader T) (c:DWORDCursor) xs : option (DWORDCursor * seq BYTE * T) :=
+  match r with
+  | readerRetn x => Some (c, xs, x)
+  | readerNext rd =>
+    if c is mkCursor p
+    then
+      if xs is x::xs
+      then runReader (rd x) (next p) xs
+      else None
+    else None
+  | readerSkip rd =>
+    if c is mkCursor p
+    then runReader rd (next p) xs
+    else None
+  | readerCursor rd =>
+    runReader (rd c) c xs
+  end.
+
+Lemma runReader_bind T U (r: Reader T) (f: T -> Reader U) :
+  forall x xs ys cursor cursor',
+  runReader r cursor xs = Some (cursor', ys, x) ->
+  runReader (readerBind r f) cursor xs = runReader (f x) cursor' ys.
+Proof. induction r.
++ move => x' xs ys c c' H. simpl in H. by injection H => -> -> ->.
++ move => x xs ys c c' H'. simpl.
+  destruct c => //.
+  destruct xs => //. simpl in H'. by apply H.
++ move => x xs ys c c' H'. simpl.
+  destruct c => //. simpl in H'. by apply IHr.
++ move => x xs ys c c' H'. simpl. simpl in H'.
+  by apply H.
+Qed.
+
+
+(*---------------------------------------------------------------------------
+   Reader type class together with BYTE, WORD, DWORD and pad instances
+  ---------------------------------------------------------------------------*)
+
+(*=readBYTE *)
+Instance readBYTE : Reader BYTE | 0 :=
+  readerNext (fun b => readerRetn b).
+(*=End *)
+
+Lemma runReader_readBYTE (p: DWORD) byte bytes :
+  runReader readBYTE p (byte::bytes) =
+  Some (next p, bytes, byte).
+Proof. done. Qed.
+
+Definition readSkip : Reader unit :=
+  readerSkip (readerRetn tt).
+
+(*=readDWORD *)
+Definition bytesToDWORD (b3 b2 b1 b0: BYTE) : DWORD :=
+  b3 ## b2 ## b1 ## b0.
+Instance readDWORD : Reader DWORD | 0 :=
+  let! b0 = readNext;
+  let! b1 = readNext;
+  let! b2 = readNext;
+  let! b3 = readNext;
+  retn (bytesToDWORD b3 b2 b1 b0).
+(*=End *)
+
+Definition bytesToQWORD (b7 b6 b5 b4 b3 b2 b1 b0: BYTE) : QWORD :=
+  b7 ## b6 ## b5 ## b4 ## b3 ## b2 ## b1 ## b0.
+Instance readQWORD : Reader QWORD | 0 :=
+  let! b0 = readNext;
+  let! b1 = readNext;
+  let! b2 = readNext;
+  let! b3 = readNext;
+  let! b4 = readNext;
+  let! b5 = readNext;
+  let! b6 = readNext;
+  let! b7 = readNext;
+  retn (bytesToQWORD b7 b6 b5 b4 b3 b2 b1 b0).
+
+Definition bytesToWORD (b1 b0: BYTE) : WORD := b1 ## b0.
+Instance readWORD: Reader WORD :=
+  let! b0 = readNext;
+  let! b1 = readNext;
+  retn (bytesToWORD b1 b0).
+
+(** This must go at a lower level/priority than [readDWORD] and [readBYTE] so it is picked up less eagerly. *)
+Instance readVWORD s : Reader (VWORD s) | 1 :=
+  match s as s return Reader (VWORD s) with
+  | OpSize1 => readBYTE
+  | OpSize2 => readWORD
+  | OpSize4 => readDWORD
+  | OpSize8 => readDWORD
+  end.
+
+Fixpoint readPad (n:nat) : Reader unit :=
+  if n is n'.+1
+  then do! readBYTE; readPad n'
+  else retn tt.
+
+Fixpoint readString (n:nat) : Reader string :=
+  if n is n'.+1
+  then let! c = readBYTE;
+       let! s = readString n';
+       retn (String (Ascii.ascii_of_nat (toNat c)) s)
+  else retn EmptyString.
+
+Fixpoint readTupleBYTE (n:nat) : Reader (n.-tuple BYTE) :=
+  if n is n'.+1
+  then let! b = readBYTE;
+       let! bs = readTupleBYTE n';
+       retn (cons_tuple b bs)
+  else retn (nil_tuple _).
+Global Existing Instance readTupleBYTE.
+
+(* Here n is the maximum number of characters to read *)
+(*Fixpoint readCString : Reader cstring :=
+  let! c = readBYTE;
+       if c == #0 then retn emptyString
+       else
+         let! s = readCString;
+         retn (cons_cstring (Ascii.ascii_of_nat (toNat c)) s).
+
+Global Existing Instance readCString.
+*)
+
+Definition readAlign (m:nat) : Reader unit :=
+  let! c = readCursor;
+  if c is mkCursor pos
+  then readPad (toNat (negB (lowWithZeroExtend m pos)))
+  else retn tt.
+
+Fixpoint readSkipPad (n:nat) : Reader unit :=
+  if n is n'.+1
+  then do! readSkip; readSkipPad n'
+  else retn tt.
+
+Definition readSkipAlign (m:nat) : Reader unit :=
+  let! c = readCursor;
+  if c is mkCursor pos
+  then readSkipPad (toNat (negB (lowWithZeroExtend m pos)))
+  else retn tt.
