src/writer.v
@@ -1,0 +1,225 @@
+(*===========================================================================
+    Syntax for writers, with instances for BYTE and DWORD
+  ===========================================================================*)
+Require Import Ssreflect.ssreflect Ssreflect.ssrfun Ssreflect.ssrbool Ssreflect.finfun Ssreflect.fintype Ssreflect.ssrnat Ssreflect.eqtype Ssreflect.seq Ssreflect.tuple.
+Require Import bitsrep bitsops cursor monad monadinst cstring.
+Require Import Coq.Logic.FunctionalExtensionality Coq.Strings.String.
+
+Set Implicit Arguments.
+Unset Strict Implicit.
+Import Prenex Implicits.
+
+(*=WriterTm *)
+Inductive WriterTm A :=
+| writerRetn (x: A)
+| writerNext (b: BYTE) (w: WriterTm A)
+| writerSkip (w: WriterTm A)
+| writerCursor (w: DWORDCursor -> WriterTm A)
+| writerFail.
+Class Writer T := getWriterTm: T -> WriterTm unit.
+(*=End *)
+Implicit Arguments writerFail [[A]].
+
+Fixpoint writerTmBind X Y (w: WriterTm X) (f: X -> WriterTm Y) : WriterTm Y :=
+  match w with
+  | writerRetn x => f x
+  | writerNext b w' => writerNext b (writerTmBind w' f)
+  | writerSkip w' => writerSkip (writerTmBind w' f)
+  | writerCursor w' => writerCursor (fun p => writerTmBind (w' p) f)
+  | writerFail => writerFail
+  end.
+
+Fixpoint writerTmSkipFree X (w: WriterTm X) :=
+match w with
+| writerRetn _ | writerFail => True
+| writerSkip _ => False
+| writerNext _ w => writerTmSkipFree w
+| writerCursor w => forall p, writerTmSkipFree (w p)
+end.
+
+Instance writerTmMonadOps : MonadOps WriterTm :=
+{ retn := @writerRetn
+; bind := writerTmBind }.
+
+Instance writerTmMonad : Monad WriterTm.
+Proof. apply Build_Monad.
+(* id_l *)
+  move => X Y x f. done.
+(* id_r *)
+  move => X. elim => //=.
+  - by move => b w' /= ->.
+  - move => w' /= IH. by apply f_equal.
+  - move => w' /= IH. apply f_equal. apply functional_extensionality => p. by rewrite IH.
+(* assoc *)
+  move => X Y Z. elim => //.
+  - move => b w' /= IH f g. by rewrite IH.
+  - move => w' /= IH f g.
+    by apply f_equal.
+  - move => w' /= IH f g. apply f_equal. apply functional_extensionality => p.
+    by rewrite IH.
+Qed.
+
+Definition getWCursor : WriterTm (DWORDCursor) := writerCursor (fun p => writerRetn p).
+Definition writeNext {T} {W: Writer T}: Writer T := W.
+
+(* Functional interpretation of writer on sequences *)
+Fixpoint runWriterTm padSkip X (w: WriterTm X) (c: DWORDCursor) : option (X * seq BYTE) :=
+  match w with
+  | writerRetn x => Some (x, nil)
+  | writerNext byte w =>
+    if c is mkCursor p
+    then
+      if runWriterTm padSkip w (next p) is Some (x, bytes) then Some (x, byte::bytes) else None
+    else None
+  | writerSkip w =>
+    if c is mkCursor p
+    then
+      if padSkip
+      then if runWriterTm padSkip w (next p) is Some (x, bytes)
+           then Some (x, #0::bytes) else None
+      else runWriterTm padSkip w (next p)
+    else None
+  | writerFail => None
+  | writerCursor w => runWriterTm padSkip (w c) c
+  end.
+
+Lemma runWriterTm_bindCursor padSkip X (w: DWORDCursor -> WriterTm X) (p: DWORD) :
+  runWriterTm padSkip (let! c = getWCursor; w c) p =
+  runWriterTm padSkip (w p) p.
+Proof. done. Qed.
+
+Lemma runWriterTm_bind padSkip X Y (w1: WriterTm X) (w2: X -> WriterTm Y) p y bytes:
+  runWriterTm padSkip (let! x = w1; w2 x) p = Some (y, bytes) ->
+  exists x p' bytes1 bytes2,
+    runWriterTm padSkip w1 p = Some (x, bytes1) /\
+    runWriterTm padSkip (w2 x) p' = Some (y, bytes2) /\
+    bytes = bytes1 ++ bytes2.
+Proof.
+  revert p bytes. induction w1 => p bytes Hrun //=.
+  - exists x, p, nil, bytes. rewrite Hrun. by eauto.
+  - simpl in Hrun. destruct p as [p|]; last done.
+    revert Hrun.
+    case Hrun': (runWriterTm _ (writerTmBind w1 w2) (next p)) => [[y' bytes']|];
+        last done.
+    move=> [Hy' Hbytes]. subst y' bytes.
+    apply IHw1 in Hrun' as [x [p' [bytes1 [bytes2 IH]]]].
+    case: IH => Hw1 [Hw2 Hbytes'] => {IHw1}.
+    do 4 eexists. rewrite Hw1. split; first done. split; first eassumption.
+    rewrite Hbytes'. done.
+  - simpl in Hrun. destruct p => //.
+    destruct padSkip.
+    * case Hrun': (runWriterTm true (writerTmBind w1 w2) (next p)) => [[y' bytes']|].
+      rewrite Hrun' in Hrun. injection Hrun => [H1 H2]. subst.
+      specialize (IHw1 (next p) _ Hrun').
+      destruct IHw1 as [x [p' [bytes1 [bytes2 [H1 [H2 H3]]]]]].
+      do 4 eexists. rewrite H1. split; first done. split; first eassumption. by subst.
+      by rewrite Hrun' in Hrun.
+    * by apply: IHw1.
+  - simpl in Hrun.
+    apply H in Hrun as [x [p' [bytes1 [bytes2 IH]]]].
+    case: IH => Hw1 [Hw2 Hbytes'] => {H}.
+    eauto 10.
+Qed.
+
+Definition runWriter padSkip T (w: Writer T) (c: DWORDCursor) (x: T): option (seq BYTE) :=
+  let! (_, bytes) = runWriterTm padSkip (w x) c;
+  retn bytes.
+
+(*---------------------------------------------------------------------------
+   Writer type class together with BYTE, WORD, DWORD and pad instances
+  ---------------------------------------------------------------------------*)
+
+(*=writeDWORD *)
+Instance writeBYTE : Writer BYTE | 0 :=
+  fun b => writerNext b (writerRetn tt).
+Instance writeDWORD : Writer DWORD | 0 := fun d =>
+  let: (b3,b2,b1,b0) := split4 8 8 8 8 d in
+  do! writeBYTE b0;
+  do! writeBYTE b1;
+  do! writeBYTE b2;
+  do! writeBYTE b3;
+  retn tt.
+(*=End *)
+
+Instance writeQWORD : Writer QWORD | 0 := fun q =>
+  let: (b7,b6,b5,b4,b3,b2,b1,b0) := split8 8 8 8 8 8 8 8 8 q in
+  do! writeBYTE b0;
+  do! writeBYTE b1;
+  do! writeBYTE b2;
+  do! writeBYTE b3;
+  do! writeBYTE b4;
+  do! writeBYTE b5;
+  do! writeBYTE b6;
+  do! writeBYTE b7;
+  retn tt.
+
+Instance writeWORD : Writer WORD := fun w =>
+  let: (b1,b0) := split2 8 8 w in
+  do! writeNext b0;
+  do! writeNext b1;
+  retn tt.
+
+(** This must go at a lower level/priority than [writeDWORD] and [writeBYTE] so it is picked up less eagerly. *)
+(*Instance writeVWORD s : Writer (VWORD s) | 1 :=
+  match s as s return Writer (VWORD s) with
+  | OpSize1 => writeBYTE
+  | OpSize2 => writeWORD
+  | OpSize4 => writeDWORD
+  | OpSize8 => writeQWORD
+  end.
+Implicit Arguments writeDWORDorBYTE [].
+*)
+
+Instance writeSkipBYTE : Writer unit :=
+  fun _ => writerSkip (writerRetn tt).
+
+Fixpoint writePadWith (b: BYTE) m : Writer unit :=
+  fun _ =>
+  if m is m'.+1
+  then do! writeBYTE b; writePadWith b m' tt
+  else retn tt.
+
+Fixpoint writeSkipBy m : Writer unit :=
+  fun _ =>
+  if m is m'.+1
+  then do! writeSkipBYTE tt; writeSkipBy m' tt
+  else retn tt.
+
+Definition writePad := writePadWith #0.
+
+Definition writeAlignWith b (m:nat) : Writer unit := fun _ =>
+  let! c = getWCursor;
+  if c is mkCursor pos
+  then writePadWith b (toNat (negB (lowWithZeroExtend m pos))) tt
+  else retn tt.
+
+Definition writeAlign := writeAlignWith #0.
+
+Definition writeSkipAlign (m:nat) : Writer unit := fun _ =>
+  let! c = getWCursor;
+  if c is mkCursor pos
+  then writeSkipBy (toNat (negB (lowWithZeroExtend m pos))) tt
+  else retn tt.
+
+
+Fixpoint writeTupleBYTE (m:nat) : Writer (m.-tuple BYTE) :=
+  if m is m'.+1
+  then fun tup => do! writeBYTE (thead tup); writeTupleBYTE (behead_tuple tup)
+  else fun tup => retn tt.
+
+Global Existing Instance writeTupleBYTE.
+
+Fixpoint writeString (n:nat) : Writer string := fun s =>
+  if n is n'.+1
+  then if s is String c s'
+       then do! writeBYTE (fromNat (Ascii.nat_of_ascii c)); writeString n' s'
+       else do! writeBYTE #0; writeString n' s
+  else retn tt.
+
+Definition writeCString : Writer cstring := fun cs =>
+  (fix WS (s:string) :=
+  if s is String c s'
+  then do! writeBYTE (fromNat (Ascii.nat_of_ascii c)); WS s'
+  else writeBYTE #0) cs.
+
+Global Existing Instance writeCString.
